Simu/Cor.v
@@ -1,15 +1,16 @@
 Require cfrontend.ClightBigstep.
 Require cfrontend.Clight.
-Require Export lib.Integers.
+Require Import lib.Integers.
 
-Require Export Rustre.Common.
-Require Export Rustre.RMemory.
+Require Import Rustre.Common.
+Require Import Rustre.RMemory.
+Require Import Rustre.Nelist.
 
-Require Export Syn Sem Tra.
+Require Import Syn Sem Tra.
 
-Require Export Program.Tactics.
-Require Export List.
-Export List.ListNotations.
+Require Import Program.Tactics.
+Require Import List.
+Import List.ListNotations.
 Open Scope list_scope.
 
 Require Import LibTactics.
@@ -22,51 +23,34 @@ Section PRESERVATION.
   Variable main_node : ident.
   Variable prog: program.
   Variable tprog: Clight.program.
-  Variable c_main: class.
-  Variable cls_main: list class.
-  
+   
   (* Let ge := globalenv prog. *)
   Let tge := Clight.globalenv tprog.
   
   Hypothesis TRANSL: translate prog main_node = Errors.OK tprog.    
   (* Hypothesis WF: well_formed prog. *)
-  Hypothesis MAINNODE: find_class main_node prog = Some (c_main, cls_main).
+  (* Hypothesis MAINNODE: find_class main_node prog = Some (c_main, cls_main). *)
 
-  Lemma build_co_ok:
-    Ctypes.build_composite_env (map translate_class prog) = Errors.OK (Clight.genv_cenv tge).
-  Proof.
-    unfold translate in TRANSL.
-    rewrite MAINNODE in TRANSL.
-    unfold Clight.make_program in TRANSL.
-    revert TRANSL.
-    generalize (Clight.make_program_obligation_1
-                  (map translate_class prog)
-                  [(main_id,
-                    make_main
-                      (translate_stmt main_node
-                                      (c_step c_main))
-                      (c_vars c_main))] 
-                  [] main_id).
-    generalize (eq_refl (Ctypes.build_composite_env (map translate_class prog))).
-    intros H1 H2.
-    simpl in H2.
-    admit.
-  Qed.
+  (* Lemma build_co_ok: *)
+  (*   Ctypes.build_composite_env (map translate_class prog) = Errors.OK (Clight.genv_cenv tge). *)
+  (* Proof. *)
+  (*   admit. *)
+  (* Qed. *)
   
   Definition chunk_of_typ ty := AST.chunk_of_type (Ctypes.typ_of_type ty).
   Definition pointer_of_node node := pointer_of (type_of_inst node).
   
-  Definition main_fun :=
-    Clight.mkfunction Ctypes.type_int32s AST.cc_default []
-                      c_main.(c_vars)
-                          []
-                          (translate_stmt main_node c_main.(c_step)).
+  (* Definition main_fun := *)
+  (*   Clight.mkfunction Ctypes.type_int32s AST.cc_default [] *)
+  (*                     c_main.(c_vars) *)
+  (*                         [] *)
+  (*                         (translate_stmt main_node c_main.(c_step)). *)
   
   Lemma type_pres:
-    forall e, Clight.typeof (translate_exp main_node e) = typeof e.
+    forall c e, Clight.typeof (translate_exp c.(c_name) e) = typeof e.
   Proof.
-    induction e; simpl; try reflexivity.
-    destruct c; simpl; reflexivity.
+    induction e as [| |cst]; simpl; try reflexivity.
+    destruct cst; simpl; reflexivity.
   Qed.
 
   Definition valid_val (v: val) (t: typ): Prop :=
@@ -85,68 +69,73 @@ Section PRESERVATION.
       (discriminates || contradiction || auto).
   Qed.
 
-  Inductive well_formed_exp: exp -> Prop :=
+  Inductive well_formed_exp (c: class): exp -> Prop :=
   | wf_var: forall x ty,
-      In (x, ty) c_main.(c_vars) ->
+      In (x, ty) c.(c_vars) ->
       x <> self_id ->
-      well_formed_exp (Var x ty)
+      well_formed_exp c (Var x ty)
   | wf_state: forall x ty,
-      In (x, ty) c_main.(c_mems) ->
-      well_formed_exp (State x ty)
-  | wf_const: forall c ty,
-      well_formed_exp (Const c ty).
+      In (x, ty) c.(c_mems) ->
+      well_formed_exp c (State x ty)
+  | wf_const: forall cst ty,
+      well_formed_exp c (Const cst ty).
 
-  Inductive well_formed_stmt (S: state): stmt -> Prop :=
+  Inductive well_formed_stmt (c: class) (S: state): stmt -> Prop :=
   | wf_assign: forall x e v,
-      In (x, typeof e) c_main.(c_vars) ->
+      In (x, typeof e) c.(c_vars) ->
       x <> self_id ->
-      well_formed_exp e ->
+      well_formed_exp c e ->
       exp_eval S e v ->
       valid_val v (typeof e) ->
       v = Values.Val.load_result (chunk_of_typ (typeof e)) v ->
-      well_formed_stmt S (Assign x e)
+      well_formed_stmt c S (Assign x e)
   | wf_assignst: forall x e v,
-      In (x, typeof e) c_main.(c_mems) ->
+      In (x, typeof e) c.(c_mems) ->
       x <> self_id ->
-      well_formed_exp e ->
+      well_formed_exp c e ->
       exp_eval S e v ->
       valid_val v (typeof e) ->
       v = Values.Val.load_result (chunk_of_typ (typeof e)) v ->
-      well_formed_stmt S (AssignSt x e)
+      well_formed_stmt c S (AssignSt x e)
   | wf_ite: forall e s1 s2,
-      well_formed_exp e ->
-      well_formed_stmt S s1 ->
-      well_formed_stmt S s2 ->
-      well_formed_stmt S (Ifte e s1 s2)
+      well_formed_exp c e ->
+      well_formed_stmt c S s1 ->
+      well_formed_stmt c S s2 ->
+      well_formed_stmt c S (Ifte e s1 s2)
   | wf_comp: forall S' s1 s2,
-      well_formed_stmt S s1 ->
-      stmt_eval S s1 S' ->
-      well_formed_stmt S' s2 ->
-      well_formed_stmt S (Comp s1 s2)
+      well_formed_stmt c S s1 ->
+      stmt_eval prog S s1 S' ->
+      well_formed_stmt c S' s2 ->
+      well_formed_stmt c S (Comp s1 s2)
+  | wf_step: forall y ty clsid o es vs,
+      Nelist.Forall (well_formed_exp c) es ->
+      Nelist.Forall2 (exp_eval S) es vs ->
+      Nelist.Forall2 (fun (e : exp) (v : val) => valid_val v (typeof e)) es vs ->
+      well_formed_stmt c S (Step_ap y ty clsid o es)
   | wf_skip: 
-      well_formed_stmt S Skip.
+      well_formed_stmt c S Skip.
 
-  Definition compat_venv (S: state) (env: Clight.env) (m: Memory.Mem.mem):  Prop :=
+  Definition compat_venv (c: class) (S: state) (env: Clight.env) (m: Memory.Mem.mem):  Prop :=
     forall x v t,
       find_var x S v ->
-      In (x, t) c_main.(c_vars) ->
+      In (x, t) c.(c_vars) ->
       exists loc,
         Maps.PTree.get x env = Some (loc, t)
         /\ Memory.Mem.load (chunk_of_typ t) m loc 0 = Some v
         /\ valid_val v t.
 
-  Definition compat_menv (S: state) (env: Clight.env) (m: Memory.Mem.mem):  Prop :=
+  Definition compat_menv (c: class) (S: state) (env: Clight.env) (m: Memory.Mem.mem):  Prop :=
     forall x v t,
       find_field x S v ->
-      In (x, t) c_main.(c_mems) ->
+      In (x, t) c.(c_mems) ->
       exists co loc' loc ofs delta,
         Ctypes.field_offset (Clight.genv_cenv tge) x (Ctypes.co_members co) = Errors.OK delta
         /\ Memory.Mem.load (chunk_of_typ t) m loc (Int.unsigned (Int.add ofs (Int.repr delta))) = Some v
         /\ valid_val v t
-        /\ Maps.PTree.get main_node (Clight.genv_cenv tge) = Some co 
-        /\ Maps.PTree.get self_id env = Some (loc', pointer_of_node main_node)
-        /\ Memory.Mem.load (chunk_of_typ (pointer_of_node main_node)) m loc' 0 = Some (Values.Vptr loc ofs)
-        /\ Ctypes.access_mode (pointer_of_node main_node) = Ctypes.By_value (chunk_of_typ (pointer_of_node main_node)).
+        /\ Maps.PTree.get c.(c_name) (Clight.genv_cenv tge) = Some co 
+        /\ Maps.PTree.get self_id env = Some (loc', pointer_of_node c.(c_name))
+        /\ Memory.Mem.load (chunk_of_typ (pointer_of_node c.(c_name))) m loc' 0 = Some (Values.Vptr loc ofs)
+        /\ Ctypes.access_mode (pointer_of_node c.(c_name)) = Ctypes.By_value (chunk_of_typ (pointer_of_node c.(c_name))).
 
   Remark valid_val_implies_access:
     forall v t, valid_val v t -> Ctypes.access_mode t = Ctypes.By_value (chunk_of_typ t).
@@ -156,15 +145,15 @@ Section PRESERVATION.
   Hint Resolve valid_val_implies_access.
   
   Lemma expr_eval_simu:
-    forall S exp v e le m,
-      compat_venv S e m ->
-      compat_menv S e m ->
-      well_formed_exp exp ->
+    forall c S exp v e le m,
+      compat_venv c S e m ->
+      compat_menv c S e m ->
+      well_formed_exp c exp ->
       exp_eval S exp v ->
-      Clight.eval_expr tge e le m (translate_exp main_node exp) v.
+      Clight.eval_expr tge e le m (translate_exp c.(c_name) exp) v.
   Proof.
-    intros S exp;
-    induction exp as [| |c];
+    intros c S exp;
+    induction exp as [| |cst];
     introv Hvenv Hmenv Hwf Heval;
     inverts Heval; inverts Hwf; simpl.
 
@@ -176,7 +165,7 @@ Section PRESERVATION.
     - edestruct Hmenv; destruct_conjs; eauto.
       eapply Clight.eval_Elvalue.
       + eapply Clight.eval_Efield_struct
-        with (id:=main_node) (att:=Ctypes.noattr); eauto.
+        with (id:=c.(c_name)) (att:=Ctypes.noattr); eauto.
         eapply Clight.eval_Elvalue. 
         * apply Clight.eval_Ederef. 
           eapply Clight.eval_Elvalue, Clight.deref_loc_value; eauto.
@@ -184,25 +173,41 @@ Section PRESERVATION.
       + apply* Clight.deref_loc_value.
 
     (* Const c ty : "c" *)
-    - destruct c; constructor.
+    - destruct cst; constructor.
+  Qed.
+
+  Lemma exprs_eval_simu:
+    forall c S es es' vs e le m,
+      compat_venv c S e m ->
+      compat_menv c S e m ->
+      Nelist.Forall (well_formed_exp c) es ->
+      Nelist.Forall2 (fun e v => valid_val v (typeof e)) es vs ->
+      Nelist.Forall2 (exp_eval S) es vs ->
+      es' = nelist2list (Nelist.map (translate_exp c.(c_name)) es) ->
+      Clight.eval_exprlist tge e le m es' (list_type_to_typelist (map Clight.typeof es')) (nelist2list vs).
+  Proof.
+    Hint Constructors Clight.eval_exprlist.
+    introv Hvenv Hmenv Hwf Hvalid Hev Heq; subst es';
+    induction Hev; inverts Hwf; inverts Hvalid; econstructor;
+    (apply* expr_eval_simu || (rewrite type_pres; apply* sem_cast_same) || eauto).
   Qed.
   
-  Definition compat_vars (e: Clight.env) (m: Memory.Mem.mem): Prop :=
+  Definition compat_vars (c: class) (e: Clight.env) (m: Memory.Mem.mem): Prop :=
     forall x t,
-      In (x, t) c_main.(c_vars) ->
+      In (x, t) c.(c_vars) ->
       exists loc,
         Maps.PTree.get x e = Some (loc, t)
         /\ Memory.Mem.valid_access m (chunk_of_typ t) loc 0 Memtype.Writable.
 
-  Definition compat_fields (env: Clight.env) (m: Memory.Mem.mem): Prop :=
+  Definition compat_fields (c: class) (env: Clight.env) (m: Memory.Mem.mem): Prop :=
     forall x t,
-      In (x, t) c_main.(c_mems) ->
+      In (x, t) c.(c_mems) ->
       exists co loc' loc ofs delta,
         Ctypes.field_offset (Clight.genv_cenv tge) x (Ctypes.co_members co) = Errors.OK delta
         /\ In (x, t) (Ctypes.co_members co)
-        /\ Maps.PTree.get main_node (Clight.genv_cenv tge) = Some co
-        /\ Maps.PTree.get self_id env = Some (loc', pointer_of_node main_node)
-        /\ Memory.Mem.load (chunk_of_typ (pointer_of_node main_node)) m loc' 0 = Some (Values.Vptr loc ofs)
+        /\ Maps.PTree.get c.(c_name) (Clight.genv_cenv tge) = Some co
+        /\ Maps.PTree.get self_id env = Some (loc', pointer_of_node c.(c_name))
+        /\ Memory.Mem.load (chunk_of_typ (pointer_of_node c.(c_name))) m loc' 0 = Some (Values.Vptr loc ofs)
         /\ Memory.Mem.valid_access m (chunk_of_typ t) loc (Int.unsigned (Int.add ofs (Int.repr delta))) Memtype.Writable.
 
   Definition nodup_env (e: Clight.env) :=
@@ -217,16 +222,16 @@ Section PRESERVATION.
       In (x, t') (Ctypes.co_members co) ->
       t' = t.
 
-  Definition nodup_vars :=
+  Definition nodup_vars (c: class) :=
     forall x t t',
-      In (x, t) c_main.(c_vars) ->
-      In (x, t') c_main.(c_vars) ->
+      In (x, t) c.(c_vars) ->
+      In (x, t') c.(c_vars) ->
       t' = t.
 
-   Definition nodup_mems :=
+   Definition nodup_mems (c: class) :=
     forall x t t',
-      In (x, t) c_main.(c_mems) ->
-      In (x, t') c_main.(c_mems) ->
+      In (x, t) c.(c_mems) ->
+      In (x, t') c.(c_mems) ->
       t' = t.
   
   Remark find_add:
@@ -272,21 +277,21 @@ Section PRESERVATION.
     apply* mfind_mem_gso.
   Qed.
   
-  Definition mem_sep (e: Clight.env) (m: Memory.Mem.mem) :=
+  Definition mem_sep (c: class) (e: Clight.env) (m: Memory.Mem.mem) :=
     forall x loc t (* co x' *) ofs (* delta t' *) loc' (* v *) loc'',
-      In (x, t) c_main.(c_vars) -> 
+      In (x, t) c.(c_vars) -> 
       Maps.PTree.get x e = Some (loc, t) ->
-      Maps.PTree.get self_id e = Some (loc'', pointer_of_node main_node) ->
-      (* Maps.PTree.get main_node (Clight.genv_cenv tge) = Some co -> *)
+      Maps.PTree.get self_id e = Some (loc'', pointer_of_node c.(c_name)) ->
+      (* Maps.PTree.get c.(c_name) (Clight.genv_cenv tge) = Some co -> *)
       (* Ctypes.field_offset (Clight.genv_cenv tge) x' (Ctypes.co_members co) = Errors.OK delta -> *)
       (* Memory.Mem.load (chunk_of_typ t') m loc' (Int.unsigned (Int.add ofs (Int.repr delta))) = Some v -> *)
-      Memory.Mem.load (chunk_of_typ (pointer_of_node main_node)) m loc'' 0 = Some (Values.Vptr loc' ofs) ->
+      Memory.Mem.load (chunk_of_typ (pointer_of_node c.(c_name))) m loc'' 0 = Some (Values.Vptr loc' ofs) ->
       loc <> loc'.
 
-  Definition self_sep (e: Clight.env) (m: Memory.Mem.mem) :=
+  Definition self_sep (c: class) (e: Clight.env) (m: Memory.Mem.mem) :=
     forall loc ofs loc',
-      Maps.PTree.get self_id e = Some (loc', pointer_of_node main_node) ->
-      Memory.Mem.load (chunk_of_typ (pointer_of_node main_node)) m loc' 0 = Some (Values.Vptr loc ofs) ->
+      Maps.PTree.get self_id e = Some (loc', pointer_of_node c.(c_name)) ->
+      Memory.Mem.load (chunk_of_typ (pointer_of_node c.(c_name))) m loc' 0 = Some (Values.Vptr loc ofs) ->
       loc <> loc'.
 
   Definition fields_sep (m: Memory.Mem.mem) :=
@@ -305,29 +310,29 @@ Section PRESERVATION.
          (Int.unsigned (Int.add ofs (Int.repr delta')))).
         
   Lemma compat_assign_pres:
-    forall S env m loc x e v,
-      compat_venv S env m ->
-      compat_menv S env m ->
-      compat_vars env m ->
-      compat_fields env m ->
-      mem_sep env m ->
-      self_sep env m ->
+    forall c S env m loc x e v,
+      compat_venv c S env m ->
+      compat_menv c S env m ->
+      compat_vars c env m ->
+      compat_fields c env m ->
+      mem_sep c env m ->
+      self_sep c env m ->
       nodup_env env ->
-      nodup_vars ->
+      nodup_vars c ->
       Maps.PTree.get x env = Some (loc, typeof e) ->
-      In (x, typeof e) c_main.(c_vars) ->
+      In (x, typeof e) c.(c_vars) ->
       v = Values.Val.load_result (chunk_of_typ (typeof e)) v ->
       valid_val v (typeof e) ->
       x <> self_id ->
       Memory.Mem.valid_access m (chunk_of_typ (typeof e)) loc 0 Memtype.Writable ->
       exp_eval S e v ->
       exists m', Memory.Mem.store (chunk_of_typ (typeof e)) m loc 0 v = Some m' 
-            /\ compat_venv (update_var x S v) env m'
-            /\ compat_menv S env m'
-            /\ compat_vars env m' 
-            /\ compat_fields env m' 
-            /\ mem_sep env m'
-            /\ self_sep env m'.
+            /\ compat_venv c (update_var x S v) env m'
+            /\ compat_menv c S env m'
+            /\ compat_vars c env m' 
+            /\ compat_fields c env m' 
+            /\ mem_sep c env m'
+            /\ self_sep c env m'.
   Proof.
     intros ** Hvenv Hmenv Hvars Hfields Hsep Hself_sep Hnodupenv Hnodupvars Hget Hin Hloadres ? ? ? ?.
     edestruct Memory.Mem.valid_access_store with (v:=v) as [m']; eauto. 
@@ -389,33 +394,33 @@ Section PRESERVATION.
   Qed.
 
    Lemma compat_stassign_pres:
-    forall S env m x e v co loc loc' ofs delta,
-      compat_venv S env m ->
-      compat_menv S env m ->
-      compat_vars env m ->
-      compat_fields env m ->
-      mem_sep env m ->
-      self_sep env m ->
+    forall c S env m x e v co loc loc' ofs delta,
+      compat_venv c S env m ->
+      compat_menv c S env m ->
+      compat_vars c env m ->
+      compat_fields c env m ->
+      mem_sep c env m ->
+      self_sep c env m ->
       fields_sep m ->
-      nodup_mems ->
+      nodup_mems c ->
       In (x, (typeof e)) (Ctypes.co_members co) ->
       Ctypes.field_offset tge.(Clight.genv_cenv) x (Ctypes.co_members co) = Errors.OK delta ->
-      Maps.PTree.get main_node (Clight.genv_cenv tge) = Some co ->
-      Maps.PTree.get self_id env = Some (loc', pointer_of_node main_node) ->
-      Memory.Mem.load (chunk_of_typ (pointer_of_node main_node)) m loc' 0 = Some (Values.Vptr loc ofs) ->
-      In (x, typeof e) c_main.(c_mems) ->
+      Maps.PTree.get c.(c_name) (Clight.genv_cenv tge) = Some co ->
+      Maps.PTree.get self_id env = Some (loc', pointer_of_node c.(c_name)) ->
+      Memory.Mem.load (chunk_of_typ (pointer_of_node c.(c_name))) m loc' 0 = Some (Values.Vptr loc ofs) ->
+      In (x, typeof e) c.(c_mems) ->
       v = Values.Val.load_result (chunk_of_typ (typeof e)) v ->
       valid_val v (typeof e) ->
      Memory.Mem.valid_access m (chunk_of_typ (typeof e)) loc (Int.unsigned (Int.add ofs (Int.repr delta))) Memtype.Writable ->
       exp_eval S e v ->
       exists m',
         Memory.Mem.store (chunk_of_typ (typeof e)) m loc (Int.unsigned (Int.add ofs (Int.repr delta))) v = Some m'
-        /\ compat_venv S env m'
-        /\ compat_menv (update_field x S v) env m'
-        /\ compat_vars env m'
-        /\ compat_fields env m'
-        /\ mem_sep env m'
-        /\ self_sep env m'.
+        /\ compat_venv c S env m'
+        /\ compat_menv c (update_field x S v) env m'
+        /\ compat_vars c env m'
+        /\ compat_fields c env m'
+        /\ mem_sep c env m'
+        /\ self_sep c env m'.
   Proof.
     intros ** Hvenv Hmenv Hvars Hfields Hsep Hself_sep Hfields_sep Hnodupmems Hmembers Hoffset Hmain Hself Hloadptr Hin Hloadres ? ? ?.
     edestruct Memory.Mem.valid_access_store with (v:=v) as [m']; eauto. 
@@ -484,9 +489,9 @@ Section PRESERVATION.
   Qed.
 
 Remark ifte_translate:
-    forall (b: bool) s1 s2,
-      translate_stmt main_node (if b then s1 else s2) =
-      if b then (translate_stmt main_node s1) else (translate_stmt main_node s2).
+    forall c temp (b: bool) s1 s2,
+      translate_stmt temp c.(c_name) (if b then s1 else s2) =
+      if b then (translate_stmt temp c.(c_name) s1) else (translate_stmt temp c.(c_name) s2).
   Proof.
     now destruct b.
   Qed.  
@@ -497,43 +502,79 @@ Remark ifte_translate:
 
   Definition c_state := (Clight.env * Clight.temp_env * Memory.Mem.mem)%type.
    
-  Inductive match_states_bigbig (S: state): c_state -> Prop :=
+  Inductive match_states_bigbig (c: class) (S: state): c_state -> Prop :=
     intro_state_bigbig: forall e le m,
       (* state correspondance *)
-      compat_venv S e m ->     
-      compat_menv S e m ->
+      compat_venv c S e m ->     
+      compat_menv c S e m ->
       
       (* Clight state well defined *)
-      compat_vars e m ->
-      compat_fields e m ->
+      compat_vars c e m ->
+      compat_fields c e m ->
 
       (* Clight side separation *)
-      mem_sep e m ->
-      self_sep e m ->
+      mem_sep c e m ->
+      self_sep c e m ->
       fields_sep m ->
       nodup_env e ->
 
       (* Minimp side separation *)
-      nodup_vars ->
-      nodup_mems ->
-      match_states_bigbig S (e, le, m).
+      nodup_vars c ->
+      nodup_mems c ->
+      match_states_bigbig c S (e, le, m).
 
   Hint Constructors match_states_bigbig.
 
+  Definition empty_temp_env: Clight.temp_env := Maps.PTree.empty val.
+      
+  Inductive unique_temp: Clight.temp_env -> option (ident * typ) -> Prop :=
+  | unique_empty:
+      unique_temp empty_temp_env None
+  | unique_singleton: forall le x v ty,
+      Maps.PTree.elements le = [(x, v)] -> 
+      unique_temp le (Some (x, ty)).
+  
   Theorem simu_bigbig:
-    forall S1 s S2,
-      well_formed_stmt S1 s ->
-      stmt_eval S1 s S2 ->
-      forall e1 le1 m1,
-        match_states_bigbig S1 (e1, le1, m1) ->
+    forall c S1 s S2,
+      well_formed_stmt c S1 s ->
+      stmt_eval prog S1 s S2 ->
+      forall e1 le1 m1 temp,
+        (* unique_temp le1 temp -> *)
+        match_states_bigbig c S1 (e1, le1, m1) ->
         exists le2 m2 t,
-          ClightBigstep.exec_stmt tge e1 le1 m1 (translate_stmt main_node s) t le2 m2 ClightBigstep.Out_normal
-          /\ match_states_bigbig S2 (e1, le2, m2).
+          ClightBigstep.exec_stmt tge e1 le1 m1
+                                  (snd (translate_stmt temp c.(c_name) s))
+                                  t le2 m2 ClightBigstep.Out_normal
+          /\ match_states_bigbig c S2 (e1, le2, m2).
   Proof.
-    introv WF EV;
-    induction EV; introv MS; inverts WF; 
+    Check stmt_eval_ind_2.
+    clear TRANSL; introv WF EV; remember prog;
+    induction EV (* using stmt_eval_ind_2 with *)
+    (* (P := fun p St1 stmt St2 => *)
+    (*         well_formed_stmt c St1 stmt -> *)
+    (*         p = prog -> *)
+    (*         forall e1 le1 m1, *)
+    (*           match_states_bigbig c St1 (e1, le1, m1) -> *)
+    (*           exists le2 m2 t, *)
+    (*             ClightBigstep.exec_stmt tge e1 le1 m1 *)
+    (*                                     (snd (translate_stmt None c.(c_name) stmt)) *)
+    (*                                     t le2 m2 ClightBigstep.Out_normal *)
+    (*             /\ match_states_bigbig c St2 (e1, le2, m2) *)
+    (* ) *)
+    (*   (P0 := fun p me clsid vs me' rv => *)
+    (*            forall p' c S1 s S2, *)
+    (*              well_formed_stmt c S1 s -> *)
+    (*              stmt_eval p' S1 s S2 -> *)
+    (*              forall e1 le1 m1, *)
+    (*                match_states_bigbig c S1 (e1, le1, m1) -> *)
+    (*                exists le2 m2 t, *)
+    (*                  ClightBigstep.exec_stmt tge e1 le1 m1 *)
+    (*                                          (snd (translate_stmt None c.(c_name) s)) *)
+    (*                                          t le2 m2 ClightBigstep.Out_normal *)
+    (*                  /\ match_states_bigbig c S2 (e1, le2, m2)) *)
+    ; introv (* UNI *) MS;  try inverts WF;
     inverts MS as Hvenv Hmenv Hvars Hfields.
-    
+
     (* Assign x e : "x = e" *)
     - app_exp_eval_det.
       edestruct Hvars; eauto.
@@ -549,7 +590,7 @@ Remark ifte_translate:
       do 3 econstructor; split*.
       apply* ClightBigstep.exec_Sassign.
       + eapply Clight.eval_Efield_struct
-        with (id:=main_node) (att:=Ctypes.noattr); eauto.
+        with (id:=c.(c_name)) (att:=Ctypes.noattr); eauto.
         apply* Clight.eval_Elvalue.  
         * apply Clight.eval_Ederef. 
           apply* Clight.eval_Elvalue.
@@ -558,20 +599,106 @@ Remark ifte_translate:
       + rewrite* type_pres.
         
     (* Ifte e s1 s2 : "if e then s1 else s2" *)
-    - edestruct IHEV; destruct_conjs; eauto;
-      [destruct b|]; auto.
-      do 3 econstructor; split*.
-      apply* ClightBigstep.exec_Sifthenelse.
-      + erewrite type_pres, bool_val_ptr; eauto. 
-      + fold translate_stmt; rewrite* <-ifte_translate.
-
+    - destruct b.
+      + edestruct IHEV with (le1:=le1) (temp:=temp) as (? & ? & ? & Step & ?); eauto. 
+        do 3 econstructor; split*.
+        simpl; destruct (translate_stmt temp (c_name c) s1);
+        destruct (translate_stmt o (c_name c) s2).
+        apply* ClightBigstep.exec_Sifthenelse. 
+        * erewrite type_pres, bool_val_ptr; eauto.
+        * eauto.
+      + simpl; destruct (translate_stmt temp (c_name c) s1) as [temp1].
+        edestruct IHEV with (le1:=le1) (temp:=temp1) as (? & ? & ? & Step & ?); eauto. 
+        do 3 econstructor; split*.
+        destruct (translate_stmt temp1 (c_name c) s2).
+        apply* ClightBigstep.exec_Sifthenelse.
+        * erewrite type_pres, bool_val_ptr; eauto.
+        * eauto.
+          
     (* Comp s1 s2 : "s1; s2" *)
-    - app_stmt_eval_det.
-      edestruct IHEV1; destruct_conjs; eauto.
-      edestruct IHEV2; destruct_conjs; eauto.
+    - subst prog0.
+      app_stmt_eval_det.
+      edestruct IHEV1 with (le1:=le1) (temp:=temp) ; destruct_conjs; eauto.
+      simpl. destruct (translate_stmt temp (c_name c) s1) as [temp1].
+      destruct (translate_stmt temp1 (c_name c) s2) eqn: E2.
+      edestruct IHEV2 with (temp:=temp1) as (? & ? & ? & Step & ?); destruct_conjs; eauto.
       do 3 econstructor; split*.
       apply* ClightBigstep.exec_Sseq_1.
-     
+      rewrite* E2 in Step.
+
+    (* Step_ap y ty clsid o [e1; ... ;en] : "y = step_clsid (&o, e1, ... , en)" *)
+    - assert (loc_f: Values.block). admit.
+      assert (Globalenvs.Genv.find_symbol (Clight.genv_genv tge) (step_id clsid) = Some loc_f). admit.
+      assert (Maps.PTree.get (step_id clsid) e1 = None). admit.
+
+      assert (loc_self: Values.block). admit.
+      assert (Maps.PTree.get self_id e1 = Some (loc_self, pointer_of_node (c_name c))). admit.
+      assert (loc_struct: Values.block). admit.
+      assert (ofs: Int.int). admit.
+      assert (Memory.Mem.loadv AST.Mint32 m1 (Values.Vptr loc_self Int.zero) = Some (Values.Vptr loc_struct ofs)). admit.
+      assert (co: Ctypes.composite). admit.
+      assert (Maps.PTree.get (c_name c) (Clight.genv_cenv tge) = Some co). admit.
+      assert (delta: Z). admit.
+      assert (Ctypes.field_offset (Clight.genv_cenv tge) o (Ctypes.co_members co) = Errors.OK delta). admit.
+
+      assert (f: Clight.function). admit.
+      assert (Globalenvs.Genv.find_funct (Clight.genv_genv tge) (Values.Vptr loc_f Int.zero) = Some (Clight.Internal f)). admit.
+
+      assert (e': Clight.env). admit.
+      assert (m': Memory.Mem.mem). admit.
+      assert (Clight.alloc_variables tge Clight.empty_env m1 (Clight.fn_params f ++ Clight.fn_vars f) e' m'). admit.
+      assert (m'': Memory.Mem.mem). admit.
+      assert (Clight.bind_parameters tge e' m' (Clight.fn_params f) (Values.Vptr loc_struct (Int.add ofs (Int.repr delta)) :: nelist2list vs0) m''). admit.
+
+      inverts H1.
+      assert (well_formed_stmt cls
+                               (omenv, adds (nefst (c_input cls)) vs v_empty) 
+                               (c_step cls)) as Hwf. admit.
+      assert (match_states_bigbig cls
+                                  (omenv, adds (nefst (c_input cls)) vs v_empty) 
+                                  (e', Clight.create_undef_temps (Clight.fn_temps f), m'')) as Hms. admit.
+      assert (Clight.fn_body f = snd (translate_stmt None (c_name cls) (c_step cls))) as Htr. admit.
+      
+        do 3 econstructor; split*.
+      eapply ClightBigstep.exec_Sseq_1.
+      + 
+        
+        eapply ClightBigstep.exec_Scall.
+        * simpl; eauto.
+        *{ eapply Clight.eval_Elvalue; simpl.
+           - apply* Clight.eval_Evar_global.
+           - apply* Clight.deref_loc_reference.
+         }
+        *{ econstructor.
+           - eapply Clight.eval_Eaddrof.
+             eapply Clight.eval_Efield_struct
+             with (id:=c.(c_name)) (att:=Ctypes.noattr); eauto.
+             apply* Clight.eval_Elvalue.  
+             + apply Clight.eval_Ederef.
+               apply* Clight.eval_Elvalue.
+               apply Clight.deref_loc_value with (chunk:=AST.Mint32); eauto.
+             + apply* Clight.deref_loc_copy.                
+           - eapply sem_cast_same.
+             unfold valid_val. splits.
+             + reflexivity.
+             + discriminate.
+             + now simpl.
+           - apply* exprs_eval_simu.
+         }
+        * eauto.
+        * admit.
+        *{ apply* ClightBigstep.eval_funcall_internal.
+           - admit.
+           - rewrite Htr.
+             (* specializes IHEV Hwf H22 Hms. *)
+             (* edestruct IHEV as (le2 & m2 & t & Hexec & Hms'); eauto. *)
+             skip.
+           - skip.
+           - skip.
+         }
+      + skip.
+      + skip.
+
     (* Skip : "skip" *)
     - do 3 econstructor; split*.
       eapply ClightBigstep.exec_Sskip.
